<?xml version="1.0" encoding="UTF-8"?>

<!--pretext-->
    <!--article xml:id="notes"-->
        <section xml:id="angle-sum-apps">
        <title>Applications of the Angle Sum Identities</title>
        <p>
            In class yesterday we did an activity to derive the first of the identities in the following:
            <paragraphs xml:id="angle-sum-identities">
  <title>The Angle Sum Identities</title>
    <p>
      If <m>\theta</m> and <m>\phi</m> are angles, then we have
      <md>
        <mrow>\sin(\theta+\phi) \amp = \sin(\theta)\cos(\phi) + \cos(\theta)\sin(\phi) </mrow>
        <mrow>\sin(\theta-\phi) \amp = \sin(\theta)\cos(\phi) - \cos(\theta)\sin(\phi) </mrow>
        <mrow>\cos(\theta+\phi)\amp = \cos(\theta)\cos(\phi) - \sin(\theta)\sin(\phi)  </mrow>
        <mrow>\cos(\theta-\phi)\amp = \cos(\theta)\cos(\phi) + \sin(\theta)\sin(\phi)  </mrow>
      </md>
    </p>
</paragraphs> 
            
            
            
            Now we will use these identities for some problems that come up in later applied math courses.  
        </p>




        <subsection xml:id="single-sinusoid">
            <title>Sums of Sinusoids with the Same Period</title>
        <p>
            In the mathematical description of oscillating objects, one frequently encounters functions of the form
            <me>
                f(t) = c_1\cos(Bt) + c_2\sin(Bt),
            </me>
            where <m>c_1</m> and <m>c_2</m> are constants. This is a periodic function with period <m>P = \frac{2\pi}{B}</m>, but we would like to know its amplitude too. To do so, we can write it in the form
            <me>
                f(t) = c_1\cos(Bt) + c_2\sin(Bt) = A\sin(Bt + \phi)
            </me>
            for some constants <m>A</m> and <m>\phi</m>. To see how, let's do an example.
        </p>
        <example>
            <statement>
                <p>
                    Let <m>f(t) = 3\cos(7t) + 2\sin(7t)</m>. To write in the form <m>f(t) = A\sin(7t + \phi)</m>, we expand the given form using the angle sum identity for sine.
                    <md>
                        <mrow> 3\cos(7t) + 2\sin(7t) \amp = A\sin(7t + \phi)</mrow>
                        <mrow> \amp = A\cos(7t)\sin(\phi) + A\sin(7t)\cos(\phi). </mrow>
                    </md>
                    Equating coefficients of <m>\cos(7t)</m> and <m>\sin(7t)</m>, we have
                    <md>
                        <mrow> 3 \amp  = A\sin(\phi)</mrow>
                        <mrow> 2 \amp  = A\cos(\phi)</mrow>
                    </md>
                    Thus,
                    <me>
                        \tan(\phi) = \frac{A\sin(\phi)}{A\cos(\phi)} = \frac{3}{2}.
                    </me>
                    Then we can take <m>\phi = \tan^{-1}(1.5)\approx 0.983</m>. Also,
                    <me>
                        A^2 = A^2\sin^2(\phi) + A^2\cos(\phi) = 9 + 4. 
                    </me>  
                    So, we <m>A = \sqrt{13}</m>. Hence,
                    <me>
                       f(t) = 3\cos(7t) + 2\sin(7t) = \sqrt{13}\sin(7t + \tan^{-1}(1.5)). 
                    </me>
                </p>
            </statement>
        </example>


        <paragraphs xml:id="phase-shift">
            <title>Writing as a Single Sine</title>
            <p>
                To write, 
                <me>
                    f(t) = c_1\cos(Bt) + c_2\sin(Bt)
                </me>
                in the form
                <me>
                    f(t) = A\sin(Bt + \phi)
                </me>
                proceed as follows:
                <ol>
                    <li>
                        <p>
                            Expand <m>A\sin(Bt + \phi)</m> using the angle sum identity for sine.
                    <md>
                        <mrow> c_1\cos(Bt) + c_2\sin(Bt) \amp = A\sin(Bt + \phi)</mrow>
                        <mrow> \amp = A\cos(Bt)\sin(\phi) + A\sin(Bt)\cos(\phi). </mrow>
                    </md>
                        </p>
                    </li>
                    <li>
                        <p>
                            Match coefficients to get
                    <md>
                        <mrow> c_1 \amp  = A\sin(\phi)</mrow>
                        <mrow> c_2 \amp  = A\cos(\phi)</mrow>
                    </md>

                        </p>
                    </li>
                    <li>
                        <p>
                            Notice that <m>A^2 = c_1^2 + c_2^2</m>, so <m>A = \sqrt{c_1^2 + c_2^2}</m>.
                        </p>
                    </li>
                    <li>
                        <p>
                            Notice that <m>\tan(\phi) = \frac{c_1}{c_2}</m>. Based on the signs of <m>c_1</m> and <m>c_2</m>, decide which quadrant <m>\phi</m> can be in, and use <m>\phi = \tan^{-1}(c_1/c_2)</m> or <m>\phi = \tan^{-1}(c_1/c_2) + \pi</m>.
                        </p>
                    </li>
                </ol>
            </p>
        </paragraphs>
        
        
        
        </subsection>

        <subsection xml:id="sum-to-product">
          <title>Sum to Product Identities and Applications</title>
        <p>
            Some identities related to the angle sum identities are the following:
                        <paragraphs xml:id="sum-to-prod-identities">
  <title>Sum to Product Identities</title>
    <p>
      If <m>\theta</m> and <m>\phi</m> are angles, then we have
      <md>
        <mrow>\sin(a) + \sin(b) \amp = 2\sin\left(\frac{a+b}{2}\right)\cos\left(\frac{a-b}{2}\right) </mrow>
        <mrow>\sin(a) - \sin(b) \amp = 2\cos\left(\frac{a+b}{2}\right)\sin\left(\frac{a-b}{2}\right) </mrow>
        <mrow>\cos(a) + \cos(b) \amp = 2\cos\left(\frac{a+b}{2}\right)\cos\left(\frac{a-b}{2}\right) </mrow>
        <mrow>\cos(a) - \cos(b) \amp = -2\sin\left(\frac{a+b}{2}\right)\sin\left(\frac{a-b}{2}\right) </mrow>
      </md>
    </p>
</paragraphs> 
        </p>
        <p>
            One use of these is to solve equations like in the following example.
        </p>
<example>
    <statement>
        <p>
            Suppose we want to solve
            <me>
                \cos(4x) + \cos(x) = 0,\ \ 0\leq x \leq \pi.
            </me>
            We apply the third identity given above to re-write the equation as
            <me>
                2\cos\left(\frac{5x}{2}\right)\cos\left(\frac{3x}{2}\right) = 0. 
            </me>
            This is a factored form, so we can set <m>\cos\left(\frac{5x}{2}\right)</m> and <m>\cos\left(\frac{3x}{2}\right)</m> equal to zero separately on the given domain to obtain
            <me>
                x = \frac{\pi}{5},\ \frac{3\pi}{5},\ \pi,\ \frac{\pi}{3}.
            </me>
            
        </p>
    </statement>
</example>

<example>
<statement>
    <p>
        One really neat application of a sum-to product formula comes when you write a sum of two sinuoidal functions with very close periods as a product. For instance,
        <me>
            \sin(2t) + \sin(2.1t) = 2\sin(2.05t)\cos(0.05t).
        </me>
        The factor <m>\sin(2.05t)</m> has a very short period while <m>\cos(0.05t)</m> has a very long period. The result is a graph that looks like the following:
            <image>
    <prefigure label = "beats-graph" xmlns="https://prefigure.org">
<diagram dimensions="(1000,1000)" margins="5">
  <definition>f(x)=sin(2*x)+sin(2.1*x)</definition>
  <coordinates bbox="(-100,-4,100,4)">
    <grid-axes xlabel="x" ylabel="y"/>
    <graph N="500" at="graph" function="f"/>
  </coordinates>

</diagram>
</prefigure>
</image>
    </p>
<p>
    What's really neat is that this allows you to <em>hear</em> this identity at work. This is what causes the wavering sound at the end of this video.
</p>
    <figure>
  <title>MIT Beats and Resonance</title>
  <video xml:id="mit-beats" youtube="pRpN9uLiouI"/>
</figure>


</statement>


</example>
        
            
        </subsection>


        </section>
    <!--/article-->
<!--/pretext-->